updating

coq/BitVectors.v
@@ -30,3 +30,308 @@ Inductive dynamic_int : Type :=
 
 Definition di_true := DI_I1 (Int1.repr 1%Z).
 Definition di_false := DI_I1 (Int1.repr 0%Z).
+
+Class VInt I : Type := {
+  (* Comparisons *)
+  eq : I -> I -> bool;
+  cmp : comparison -> I -> I -> bool;
+  cmpu : comparison -> I -> I -> bool;
+
+  (* Constants *)
+  bitwidth : nat;
+  zero : I;
+  one : I;
+
+  (* Arithmetic *)
+  add : I -> I -> I;
+  add_carry : I -> I -> I -> I;
+  add_overflow : I -> I -> I -> I;
+
+  sub : I -> I -> I;
+  sub_borrow : I -> I -> I -> I;
+  sub_overflow : I -> I -> I -> I;
+
+  mul : I -> I -> I;
+
+  divu : I -> I -> I;
+  divs : I -> I -> I;
+  modu : I -> I -> I;
+  mods : I -> I -> I;
+
+  shl : I -> I -> I;
+  shr : I -> I -> I;
+  shru : I -> I -> I;
+
+  negative : I -> I;
+
+  (* Logic *)
+  and : I -> I -> I;
+  or : I -> I -> I;
+  xor : I -> I -> I;
+
+  (* Bounds *)
+  min_signed : Z;
+  max_signed : Z;
+
+  (* Conversion *)
+  to_dint : I -> dynamic_int;
+  unsigned : I -> Z;
+  signed : I -> Z;
+
+  repr : Z -> I;
+}.
+
+Global Instance VInt1 : VInt Int1.int := {
+  (* Comparisons *)
+  eq := Int1.eq;
+  cmp := Int1.cmp;
+  cmpu := Int1.cmpu;
+
+  bitwidth := 1;
+
+  (* Constants *)
+  zero := Int1.zero;
+  one := Int1.one;
+
+  (* Arithmetic *)
+  add := Int1.add;
+  add_carry := Int1.add_carry;
+  add_overflow := Int1.add_overflow;
+
+  sub := Int1.sub;
+  sub_borrow := Int1.sub_borrow;
+  sub_overflow := Int1.sub_overflow;
+
+  mul := Int1.mul;
+
+  divu := Int1.divu;
+  divs := Int1.divs;
+  modu := Int1.modu;
+  mods := Int1.mods;
+
+  shl := Int1.shl;
+  shr := Int1.shr;
+  shru := Int1.shru;
+
+  negative := Int1.negative;
+
+  (* Logic *)
+  and := Int1.and;
+  or := Int1.or;
+  xor := Int1.xor;
+
+  (* Bounds *)
+  min_signed := Int1.min_signed;
+  max_signed := Int1.max_signed;
+
+  (* Conversion *)
+  to_dint := DI_I1;
+  unsigned := Int1.unsigned;
+  signed := Int1.signed;
+
+  repr := Int1.repr;
+}.
+
+Global Instance VInt8 : VInt Int8.int := {
+  (* Comparisons *)
+  eq := Int8.eq;
+  cmp := Int8.cmp;
+  cmpu := Int8.cmpu;
+
+  bitwidth := 8;
+
+  (* Constants *)
+  zero := Int8.zero;
+  one := Int8.one;
+
+  (* Arithmetic *)
+  add := Int8.add;
+  add_carry := Int8.add_carry;
+  add_overflow := Int8.add_overflow;
+
+  sub := Int8.sub;
+  sub_borrow := Int8.sub_borrow;
+  sub_overflow := Int8.sub_overflow;
+
+  mul := Int8.mul;
+
+  divu := Int8.divu;
+  divs := Int8.divs;
+  modu := Int8.modu;
+  mods := Int8.mods;
+
+  shl := Int8.shl;
+  shr := Int8.shr;
+  shru := Int8.shru;
+
+  negative := Int8.negative;
+
+  (* Logic *)
+  and := Int8.and;
+  or := Int8.or;
+  xor := Int8.xor;
+
+  (* Bounds *)
+  min_signed := Int8.min_signed;
+  max_signed := Int8.max_signed;
+
+  (* Conversion *)
+  to_dint := DI_I8;
+  unsigned := Int8.unsigned;
+  signed := Int8.signed;
+
+  repr := Int8.repr;
+}.
+
+Global Instance VInt16 : VInt Int16.int := {
+  (* Comparisons *)
+  eq := Int16.eq;
+  cmp := Int16.cmp;
+  cmpu := Int16.cmpu;
+
+  bitwidth := 16;
+
+  (* Constants *)
+  zero := Int16.zero;
+  one := Int16.one;
+
+  (* Arithmetic *)
+  add := Int16.add;
+  add_carry := Int16.add_carry;
+  add_overflow := Int16.add_overflow;
+
+  sub := Int16.sub;
+  sub_borrow := Int16.sub_borrow;
+  sub_overflow := Int16.sub_overflow;
+
+  mul := Int16.mul;
+
+  divu := Int16.divu;
+  divs := Int16.divs;
+  modu := Int16.modu;
+  mods := Int16.mods;
+
+  shl := Int16.shl;
+  shr := Int16.shr;
+  shru := Int16.shru;
+
+  negative := Int16.negative;
+
+  (* Logic *)
+  and := Int16.and;
+  or := Int16.or;
+  xor := Int16.xor;
+
+  (* Bounds *)
+  min_signed := Int16.min_signed;
+  max_signed := Int16.max_signed;
+
+  (* Conversion *)
+  to_dint := DI_I16;
+  unsigned := Int16.unsigned;
+  signed := Int16.signed;
+
+  repr := Int16.repr;
+}.
+
+Global Instance VInt32 : VInt Int32.int := {
+  (* Comparisons *)
+  eq := Int32.eq;
+  cmp := Int32.cmp;
+  cmpu := Int32.cmpu;
+
+  bitwidth := 32;
+
+  (* Constants *)
+  zero := Int32.zero;
+  one := Int32.one;
+
+  (* Arithmetic *)
+  add := Int32.add;
+  add_carry := Int32.add_carry;
+  add_overflow := Int32.add_overflow;
+
+  sub := Int32.sub;
+  sub_borrow := Int32.sub_borrow;
+  sub_overflow := Int32.sub_overflow;
+
+  mul := Int32.mul;
+
+  divu := Int32.divu;
+  divs := Int32.divs;
+  modu := Int32.modu;
+  mods := Int32.mods;
+
+  shl := Int32.shl;
+  shr := Int32.shr;
+  shru := Int32.shru;
+
+  negative := Int32.negative;
+
+  (* Logic *)
+  and := Int32.and;
+  or := Int32.or;
+  xor := Int32.xor;
+
+  (* Bounds *)
+  min_signed := Int32.min_signed;
+  max_signed := Int32.max_signed;
+
+  (* Conversion *)
+  to_dint := DI_I32;
+  unsigned := Int32.unsigned;
+  signed := Int32.signed;
+
+  repr := Int32.repr;
+}.
+
+Global Instance VInt64 : VInt Int64.int := {
+  (* Comparisons *)
+  eq := Int64.eq;
+  cmp := Int64.cmp;
+  cmpu := Int64.cmpu;
+
+  bitwidth := 64;
+
+  (* Constants *)
+  zero := Int64.zero;
+  one := Int64.one;
+
+  (* Arithmetic *)
+  add := Int64.add;
+  add_carry := Int64.add_carry;
+  add_overflow := Int64.add_overflow;
+
+  sub := Int64.sub;
+  sub_borrow := Int64.sub_borrow;
+  sub_overflow := Int64.sub_overflow;
+
+  mul := Int64.mul;
+
+  divu := Int64.divu;
+  divs := Int64.divs;
+  modu := Int64.modu;
+  mods := Int64.mods;
+
+  shl := Int64.shl;
+  shr := Int64.shr;
+  shru := Int64.shru;
+
+  negative := Int64.negative;
+
+  (* Logic *)
+  and := Int64.and;
+  or := Int64.or;
+  xor := Int64.xor;
+
+  (* Bounds *)
+  min_signed := Int64.min_signed;
+  max_signed := Int64.max_signed;
+
+  (* Conversion *)
+  to_dint := DI_I64;
+  unsigned := Int64.unsigned;
+  signed := Int64.signed;
+
+  repr := Int64.repr;
+}.
