coq/DynamicValue.v
@@ -6,333 +6,40 @@ From SE.Numeric Require Import Integers.
 From SE Require Import LLVMAst.
 
 Inductive dynamic_value : Type :=
-  | DV_I1 (n : int1)
-  | DV_I8 (n : int8)
-  | DV_I16 (n : int16)
-  | DV_I32 (n : int32)
-  | DV_I64 (n : int64)
+  | DV_Int (di : dynamic_int)
   | DV_Undef
   | DV_Poison
 .
 
-Class VInt I : Type := {
-  (* Comparisons *)
-  eq : I -> I -> bool;
-  cmp : comparison -> I -> I -> bool;
-  cmpu : comparison -> I -> I -> bool;
-
-  (* Constants *)
-  bitwidth : nat;
-  zero : I;
-  one : I;
-
-  (* Arithmetic *)
-  add : I -> I -> I;
-  add_carry : I -> I -> I -> I;
-  add_overflow : I -> I -> I -> I;
-
-  sub : I -> I -> I;
-  sub_borrow : I -> I -> I -> I;
-  sub_overflow : I -> I -> I -> I;
-
-  mul : I -> I -> I;
-
-  divu : I -> I -> I;
-  divs : I -> I -> I;
-  modu : I -> I -> I;
-  mods : I -> I -> I;
-
-  shl : I -> I -> I;
-  shr : I -> I -> I;
-  shru : I -> I -> I;
-
-  negative : I -> I;
-
-  (* Logic *)
-  and : I -> I -> I;
-  or : I -> I -> I;
-  xor : I -> I -> I;
-
-  (* Bounds *)
-  min_signed : Z;
-  max_signed : Z;
-
-  (* Conversion *)
-  (* TODO: remove *)
+Class ConvertToDV I : Type := {
   to_dvalue : I -> dynamic_value;
-  to_dint : I -> dynamic_int;
-  unsigned : I -> Z;
-  signed : I -> Z;
-
-  repr : Z -> I;
 }.
 
-Global Instance VInt1 : VInt Int1.int := {
-  (* Comparisons *)
-  eq := Int1.eq;
-  cmp := Int1.cmp;
-  cmpu := Int1.cmpu;
-
-  bitwidth := 1;
-
-  (* Constants *)
-  zero := Int1.zero;
-  one := Int1.one;
-
-  (* Arithmetic *)
-  add := Int1.add;
-  add_carry := Int1.add_carry;
-  add_overflow := Int1.add_overflow;
-
-  sub := Int1.sub;
-  sub_borrow := Int1.sub_borrow;
-  sub_overflow := Int1.sub_overflow;
-
-  mul := Int1.mul;
-
-  divu := Int1.divu;
-  divs := Int1.divs;
-  modu := Int1.modu;
-  mods := Int1.mods;
-
-  shl := Int1.shl;
-  shr := Int1.shr;
-  shru := Int1.shru;
-
-  negative := Int1.negative;
-
-  (* Logic *)
-  and := Int1.and;
-  or := Int1.or;
-  xor := Int1.xor;
-
-  (* Bounds *)
-  min_signed := Int1.min_signed;
-  max_signed := Int1.max_signed;
-
-  (* Conversion *)
-  to_dvalue := DV_I1;
-  to_dint := DI_I1;
-  unsigned := Int1.unsigned;
-  signed := Int1.signed;
-
-  repr := Int1.repr;
+Global Instance ConvertToDVInt1 : ConvertToDV Int1.int := {
+  to_dvalue := fun x => DV_Int (DI_I1 x);
 }.
 
-Global Instance VInt8 : VInt Int8.int := {
-  (* Comparisons *)
-  eq := Int8.eq;
-  cmp := Int8.cmp;
-  cmpu := Int8.cmpu;
-
-  bitwidth := 8;
-
-  (* Constants *)
-  zero := Int8.zero;
-  one := Int8.one;
-
-  (* Arithmetic *)
-  add := Int8.add;
-  add_carry := Int8.add_carry;
-  add_overflow := Int8.add_overflow;
-
-  sub := Int8.sub;
-  sub_borrow := Int8.sub_borrow;
-  sub_overflow := Int8.sub_overflow;
-
-  mul := Int8.mul;
-
-  divu := Int8.divu;
-  divs := Int8.divs;
-  modu := Int8.modu;
-  mods := Int8.mods;
-
-  shl := Int8.shl;
-  shr := Int8.shr;
-  shru := Int8.shru;
-
-  negative := Int8.negative;
-
-  (* Logic *)
-  and := Int8.and;
-  or := Int8.or;
-  xor := Int8.xor;
-
-  (* Bounds *)
-  min_signed := Int8.min_signed;
-  max_signed := Int8.max_signed;
-
-  (* Conversion *)
-  to_dvalue := DV_I8;
-  to_dint := DI_I8;
-  unsigned := Int8.unsigned;
-  signed := Int8.signed;
-
-  repr := Int8.repr;
+Global Instance ConvertToDVInt8 : ConvertToDV Int8.int := {
+  to_dvalue := fun x => DV_Int (DI_I8 x);
 }.
 
-Global Instance VInt16 : VInt Int16.int := {
-  (* Comparisons *)
-  eq := Int16.eq;
-  cmp := Int16.cmp;
-  cmpu := Int16.cmpu;
-
-  bitwidth := 16;
-
-  (* Constants *)
-  zero := Int16.zero;
-  one := Int16.one;
-
-  (* Arithmetic *)
-  add := Int16.add;
-  add_carry := Int16.add_carry;
-  add_overflow := Int16.add_overflow;
-
-  sub := Int16.sub;
-  sub_borrow := Int16.sub_borrow;
-  sub_overflow := Int16.sub_overflow;
-
-  mul := Int16.mul;
-
-  divu := Int16.divu;
-  divs := Int16.divs;
-  modu := Int16.modu;
-  mods := Int16.mods;
-
-  shl := Int16.shl;
-  shr := Int16.shr;
-  shru := Int16.shru;
-
-  negative := Int16.negative;
-
-  (* Logic *)
-  and := Int16.and;
-  or := Int16.or;
-  xor := Int16.xor;
-
-  (* Bounds *)
-  min_signed := Int16.min_signed;
-  max_signed := Int16.max_signed;
-
-  (* Conversion *)
-  to_dvalue := DV_I16;
-  to_dint := DI_I16;
-  unsigned := Int16.unsigned;
-  signed := Int16.signed;
-
-  repr := Int16.repr;
+Global Instance ConvertToDVInt16 : ConvertToDV Int16.int := {
+  to_dvalue := fun x => DV_Int (DI_I16 x);
 }.
 
-Global Instance VInt32 : VInt Int32.int := {
-  (* Comparisons *)
-  eq := Int32.eq;
-  cmp := Int32.cmp;
-  cmpu := Int32.cmpu;
-
-  bitwidth := 32;
-
-  (* Constants *)
-  zero := Int32.zero;
-  one := Int32.one;
-
-  (* Arithmetic *)
-  add := Int32.add;
-  add_carry := Int32.add_carry;
-  add_overflow := Int32.add_overflow;
-
-  sub := Int32.sub;
-  sub_borrow := Int32.sub_borrow;
-  sub_overflow := Int32.sub_overflow;
-
-  mul := Int32.mul;
-
-  divu := Int32.divu;
-  divs := Int32.divs;
-  modu := Int32.modu;
-  mods := Int32.mods;
-
-  shl := Int32.shl;
-  shr := Int32.shr;
-  shru := Int32.shru;
-
-  negative := Int32.negative;
-
-  (* Logic *)
-  and := Int32.and;
-  or := Int32.or;
-  xor := Int32.xor;
-
-  (* Bounds *)
-  min_signed := Int32.min_signed;
-  max_signed := Int32.max_signed;
-
-  (* Conversion *)
-  to_dvalue := DV_I32;
-  to_dint := DI_I32;
-  unsigned := Int32.unsigned;
-  signed := Int32.signed;
-
-  repr := Int32.repr;
+Global Instance ConvertToDVInt32 : ConvertToDV Int32.int := {
+  to_dvalue := fun x => DV_Int (DI_I32 x);
 }.
 
-Global Instance VInt64 : VInt Int64.int := {
-  (* Comparisons *)
-  eq := Int64.eq;
-  cmp := Int64.cmp;
-  cmpu := Int64.cmpu;
-
-  bitwidth := 64;
-
-  (* Constants *)
-  zero := Int64.zero;
-  one := Int64.one;
-
-  (* Arithmetic *)
-  add := Int64.add;
-  add_carry := Int64.add_carry;
-  add_overflow := Int64.add_overflow;
-
-  sub := Int64.sub;
-  sub_borrow := Int64.sub_borrow;
-  sub_overflow := Int64.sub_overflow;
-
-  mul := Int64.mul;
-
-  divu := Int64.divu;
-  divs := Int64.divs;
-  modu := Int64.modu;
-  mods := Int64.mods;
-
-  shl := Int64.shl;
-  shr := Int64.shr;
-  shru := Int64.shru;
-
-  negative := Int64.negative;
-
-  (* Logic *)
-  and := Int64.and;
-  or := Int64.or;
-  xor := Int64.xor;
-
-  (* Bounds *)
-  min_signed := Int64.min_signed;
-  max_signed := Int64.max_signed;
-
-  (* Conversion *)
-  to_dvalue := DV_I64;
-  to_dint := DI_I64;
-  unsigned := Int64.unsigned;
-  signed := Int64.signed;
-
-  repr := Int64.repr;
+Global Instance ConvertToDVInt64 : ConvertToDV Int64.int := {
+  to_dvalue := fun x => DV_Int (DI_I64 x);
 }.
 
-Definition dv_true := DV_I1 one.
-Definition dv_false := DV_I1 zero.
+Definition dv_true := DV_Int di_true.
+Definition dv_false := DV_Int di_false.
 
 (* TODO: compare with the latest version *)
-(* TODO: why returns DV_Undef in some cases? *)
-Definition eval_ibinop_generic {Int} `{VInt Int} (op : ibinop) (x y : Int) : dynamic_value :=
+Definition eval_ibinop_generic {Int} `{VInt Int} `{ConvertToDV Int} (op : ibinop) (x y : Int) : dynamic_value :=
   match op with
   | Add nuw nsw =>
     if orb (andb nuw (eq (add_carry x y zero) one))
@@ -340,14 +47,12 @@ Definition eval_ibinop_generic {Int} `{VInt Int} (op : ibinop) (x y : Int) : dyn
       DV_Poison
     else
       to_dvalue (add x y)
-
   | Sub nuw nsw =>
     if orb (andb nuw (eq (sub_borrow x y zero) one))
            (andb nsw (eq (sub_overflow x y zero) one)) then
       DV_Poison
     else
       to_dvalue (sub x y)
-
   | Mul nuw nsw =>
     if (bitwidth =? 1)%nat then
       to_dvalue (mul x y)
@@ -359,7 +64,6 @@ Definition eval_ibinop_generic {Int} `{VInt Int} (op : ibinop) (x y : Int) : dyn
         DV_Poison
       else
         to_dvalue res
-
   | Shl nuw nsw =>
     if (bitwidth =? 1)%nat then
       if ((unsigned y) >=? 1)%Z then DV_Undef else to_dvalue x
@@ -375,19 +79,16 @@ Definition eval_ibinop_generic {Int} `{VInt Int} (op : ibinop) (x y : Int) : dyn
         DV_Poison
       else
         to_dvalue res
-
   | UDiv ex =>
     if andb ex (negb ((unsigned x) mod (unsigned y) =? 0)%Z) then
       DV_Poison
     else
       to_dvalue (divu x y)
-
   | SDiv ex =>
     if andb ex (negb (((signed x) mod (signed y)) =? 0)%Z) then
       DV_Poison
     else
       to_dvalue (divs x y)
-
   | LShr ex =>
     if (bitwidth =? 1)%nat then
       if ((unsigned y) >=? 1)%Z then DV_Undef else to_dvalue x
@@ -399,7 +100,6 @@ Definition eval_ibinop_generic {Int} `{VInt Int} (op : ibinop) (x y : Int) : dyn
         DV_Poison
       else
         to_dvalue (shru x y)
-
   | AShr ex =>
     if (bitwidth =? 1)%nat then
       if ((unsigned y) >=? 1)%Z then DV_Undef else to_dvalue x
@@ -411,46 +111,39 @@ Definition eval_ibinop_generic {Int} `{VInt Int} (op : ibinop) (x y : Int) : dyn
        DV_Poison
      else
        to_dvalue (shr x y)
-
   | URem => to_dvalue (modu x y)
-
   | SRem => to_dvalue (mods x y)
-
   | And => to_dvalue (and x y)
-
   | Or => to_dvalue (or x y)
-
   | Xor => to_dvalue (xor x y)
-
   end
 .
 
 Definition make_bool (b : bool) : dynamic_value :=
   match b with
-  | true => DV_I1 (Int1.repr 1)
-  | false => DV_I1 (Int1.repr 0)
+  | true => dv_true
+  | false => dv_false
   end
 .
 
 Definition make_dv (bits : N) (n : Z) : option dynamic_value :=
   match bits with
-  | 1%N => Some (DV_I1 (Int1.repr n))
-  | 8%N => Some (DV_I8 (Int8.repr n))
-  | 16%N => Some (DV_I16 (Int16.repr n))
-  | 32%N => Some (DV_I32 (Int32.repr n))
-  | 64%N => Some (DV_I64 (Int64.repr n))
+  | 1%N => Some (DV_Int (DI_I1 (Int1.repr n)))
+  | 8%N => Some (DV_Int (DI_I8 (Int8.repr n)))
+  | 16%N => Some (DV_Int (DI_I16 (Int16.repr n)))
+  | 32%N => Some (DV_Int (DI_I32 (Int32.repr n)))
+  | 64%N => Some (DV_Int (DI_I64 (Int64.repr n)))
   | _ => None
   end
 .
 
-(* TODO: rename to eval_binop *)
-Fixpoint eval_ibinop (op : ibinop) (v1 v2 : dynamic_value) : option dynamic_value :=
-  match (v1, v2) with
-  | (DV_I1 n1, DV_I1 n2)
-  | (DV_I8 n1, DV_I8 n2)
-  | (DV_I16 n1, DV_I16 n2)
-  | (DV_I32 n1, DV_I32 n2)
-  | (DV_I64 n1, DV_I64 n2) => Some (eval_ibinop_generic op n1 n2)
+Fixpoint eval_ibinop (op : ibinop) (dv1 dv2 : dynamic_value) : option dynamic_value :=
+  match (dv1, dv2) with
+  | (DV_Int (DI_I1 n1),  DV_Int (DI_I1 n2))
+  | (DV_Int (DI_I8 n1),  DV_Int (DI_I8 n2))
+  | (DV_Int (DI_I16 n1), DV_Int (DI_I16 n2))
+  | (DV_Int (DI_I32 n1), DV_Int (DI_I32 n2))
+  | (DV_Int (DI_I64 n1), DV_Int (DI_I64 n2)) => Some (eval_ibinop_generic op n1 n2)
   | _ => None
   end
 .
@@ -470,18 +163,18 @@ Definition eval_icmp_generic {Int} `{VInt Int} icmp (x y : Int) : dynamic_value 
      | Sle => cmp Cle x y
      end
   then
-    DV_I1 (Int1.one)
+    dv_true
   else
-    DV_I1 (Int1.zero)
+    dv_false
 .
 
 Fixpoint eval_icmp (op : icmp) (v1 v2 : dynamic_value) : option dynamic_value :=
   match (v1, v2) with
-  | (DV_I1 n1, DV_I1 n2)
-  | (DV_I8 n1, DV_I8 n2)
-  | (DV_I16 n1, DV_I16 n2)
-  | (DV_I32 n1, DV_I32 n2)
-  | (DV_I64 n1, DV_I64 n2) => Some (eval_icmp_generic op n1 n2)
+  | (DV_Int (DI_I1 n1),  DV_Int (DI_I1 n2))
+  | (DV_Int (DI_I8 n1),  DV_Int (DI_I8 n2))
+  | (DV_Int (DI_I16 n1), DV_Int (DI_I16 n2))
+  | (DV_Int (DI_I32 n1), DV_Int (DI_I32 n2))
+  | (DV_Int (DI_I64 n1), DV_Int (DI_I64 n2)) => Some (eval_icmp_generic op n1 n2)
   | _ => None
   end
 .
@@ -492,50 +185,50 @@ Definition convert conv x t1 t2 : option dynamic_value :=
   match conv with
   | Trunc =>
     match t1, x, t2 with
-    | TYPE_I 8, DV_I8 i1, TYPE_I 1 =>
-      Some (DV_I1 (repr (unsigned i1)))
-    | TYPE_I 32, DV_I32 i1, TYPE_I 1 =>
-      Some (DV_I1 (repr (unsigned i1)))
-    | TYPE_I 32, DV_I32 i1, TYPE_I 8 =>
-      Some (DV_I8 (repr (unsigned i1)))
-    | TYPE_I 64, DV_I64 i1, TYPE_I 1 =>
-      Some (DV_I1 (repr (unsigned i1)))
-    | TYPE_I 64, DV_I64 i1, TYPE_I 8 =>
-      Some (DV_I8 (repr (unsigned i1)))
-    | TYPE_I 64, DV_I64 i1, TYPE_I 32 =>
-      Some (DV_I32 (repr (unsigned i1)))
+    | TYPE_I 8, DV_Int (DI_I8 i1), TYPE_I 1 =>
+      Some (DV_Int (DI_I1 (repr (unsigned i1))))
+    | TYPE_I 32, DV_Int (DI_I32 i1), TYPE_I 1 =>
+      Some (DV_Int (DI_I1 (repr (unsigned i1))))
+    | TYPE_I 32, DV_Int (DI_I32 i1), TYPE_I 8 =>
+      Some (DV_Int (DI_I8 (repr (unsigned i1))))
+    | TYPE_I 64, DV_Int (DI_I64 i1), TYPE_I 1 =>
+      Some (DV_Int (DI_I1 (repr (unsigned i1))))
+    | TYPE_I 64, DV_Int (DI_I64 i1), TYPE_I 8 =>
+      Some (DV_Int (DI_I8 (repr (unsigned i1))))
+    | TYPE_I 64, DV_Int (DI_I64 i1), TYPE_I 32 =>
+      Some (DV_Int (DI_I32 (repr (unsigned i1))))
     | _, _, _ => None
     end
   | Zext =>
     match t1, x, t2 with
-    | TYPE_I 1, DV_I1 i1, TYPE_I 8 =>
-      Some (DV_I8 (repr (unsigned i1)))
-    | TYPE_I 1, DV_I1 i1, TYPE_I 32 =>
-      Some (DV_I32 (repr (unsigned i1)))
-    | TYPE_I 1, DV_I1 i1, TYPE_I 64 =>
-      Some (DV_I64 (repr (unsigned i1)))
-    | TYPE_I 8, DV_I8 i1, TYPE_I 32 =>
-      Some (DV_I32 (repr (unsigned i1)))
-    | TYPE_I 8, DV_I8 i1, TYPE_I 64 =>
-      Some (DV_I64 (repr (unsigned i1)))
-    | TYPE_I 32, DV_I32 i1, TYPE_I 64 =>
-      Some (DV_I64 (repr (unsigned i1)))
+    | TYPE_I 1, DV_Int (DI_I1 i1), TYPE_I 8 =>
+      Some (DV_Int (DI_I8 (repr (unsigned i1))))
+    | TYPE_I 1, DV_Int (DI_I1 i1), TYPE_I 32 =>
+      Some (DV_Int (DI_I32 (repr (unsigned i1))))
+    | TYPE_I 1, DV_Int (DI_I1 i1), TYPE_I 64 =>
+      Some (DV_Int (DI_I64 (repr (unsigned i1))))
+    | TYPE_I 8, DV_Int (DI_I8 i1), TYPE_I 32 =>
+      Some (DV_Int (DI_I32 (repr (unsigned i1))))
+    | TYPE_I 8, DV_Int (DI_I8 i1), TYPE_I 64 =>
+      Some (DV_Int (DI_I64 (repr (unsigned i1))))
+    | TYPE_I 32, DV_Int (DI_I32 i1), TYPE_I 64 =>
+      Some (DV_Int (DI_I64 (repr (unsigned i1))))
     | _, _, _ => None
     end
   | Sext =>
     match t1, x, t2 with
-    | TYPE_I 1, DV_I1 i1, TYPE_I 8 =>
-      Some (DV_I8 (repr (signed i1)))
-    | TYPE_I 1, DV_I1 i1, TYPE_I 32 =>
-      Some (DV_I32 (repr (signed i1)))
-    | TYPE_I 1, DV_I1 i1, TYPE_I 64 =>
-      Some (DV_I64 (repr (signed i1)))
-    | TYPE_I 8, DV_I8 i1, TYPE_I 32 =>
-      Some (DV_I32 (repr (signed i1)))
-    | TYPE_I 8, DV_I8 i1, TYPE_I 64 =>
-      Some (DV_I64 (repr (signed i1)))
-    | TYPE_I 32, DV_I32 i1, TYPE_I 64 =>
-      Some (DV_I64 (repr (signed i1)))
+    | TYPE_I 1, DV_Int (DI_I1 i1), TYPE_I 8 =>
+      Some (DV_Int (DI_I8 (repr (signed i1))))
+    | TYPE_I 1, DV_Int (DI_I1 i1), TYPE_I 32 =>
+      Some (DV_Int (DI_I32 (repr (signed i1))))
+    | TYPE_I 1, DV_Int (DI_I1 i1), TYPE_I 64 =>
+      Some (DV_Int (DI_I64 (repr (signed i1))))
+    | TYPE_I 8, DV_Int (DI_I8 i1), TYPE_I 32 =>
+      Some (DV_Int (DI_I32 (repr (signed i1))))
+    | TYPE_I 8, DV_Int (DI_I8 i1), TYPE_I 64 =>
+      Some (DV_Int (DI_I64 (repr (signed i1))))
+    | TYPE_I 32, DV_Int (DI_I32 i1), TYPE_I 64 =>
+      Some (DV_Int (DI_I64 (repr (signed i1))))
     | _, _, _ => None
     end
   | Bitcast =>
